merged files

src/tactic/compute_degree.lean
@@ -3,32 +3,205 @@ Copyright (c) 2022 Damiano Testa. All rights reserved.
 Released under Apache 2.0 license as described in the file LICENSE.
 Authors: Damiano Testa
 -/
+import tactic.move_add
 import data.polynomial.degree.lemmas
 
-/-! # `compute_degree_le` a tactic for computing degrees of polynomials
+/-! # `compute_degree, compute_degree_le` tactics for computing degrees of polynomials
 
-This file defines the tactic `compute_degree_le`.
+This file defines two main tactics `compute_degree` and `compute_degree_le`.
+Applied when the goal is of the form `f.(nat_)degree = d` or `f.(nat_)degree ≤ d`, they try to
+solve it.
+They may leave side-goals, in case they are not entirely successful.
 
-Using `compute_degree_le` when the goal is of the form `f.nat_degree ≤ d`, tries to solve the goal.
-It may leave side-goals, in case it is not entirely successful.
-
-See the doc-string for more details.
+See the corresponding doc-strings for more details.
 
 ##  Future work
 
-* Deal with goals of the form `f.(nat_)degree = d` (PR #14040 does exactly this).
 * Add better functionality to deal with exponents that are not necessarily closed natural numbers.
+* It may not be hard to allow an optional argument to be passed to `compute_degree` that would
+  let the tactic know which ones are the terms of highest degree.  This would bypass the step
+  where the exponents get sorted and may make it accessible to continue with the rest of the
+  argument with minimal change.
+* Add functionality to close `monic` goals and compute `leading_coeff`s.
 * Add support for proving goals of the from `f.(nat_)degree ≠ 0`.
 * Make sure that `degree` and `nat_degree` are equally supported.
 
 ##  Implementation details
 
-We start with a goal of the form `f.(nat_)degree ≤ d`.  Recurse into `f` breaking apart sums,
-products and powers.  Take care of numerals, `C a, X (^ n), monomial a n` separately. -/
+We start with a goal of the form `f.nat_degree = d` (the case `f.nat_degree ≤ d` follows a similar,
+easier pattern).
+
+First, we focus on an elementary term of the polynomial `f` and we extract the degree in easy cases:
+if `f` is
+* `monomial n r`, then we guess `n`,
+* `C a`, then we guess `0`,
+* `polynomial.X`, then we guess `1`,
+* `X ^ n`, then we guess `n`,
+* everything else, then we guess `f.nat_degree`.
+This happens in `extract_deg_single_term`.
+
+Second, with input a product, we sum the guesses made above on each factor and add them up.
+This happens in `extract_deg_single_summand`.
+
+Third, we scan the summands of `f`, searching for one with highest guessed degree.  Here, if a
+guess is not a closed term of type `ℕ`, the tactic fails.  This could be improved, but is not
+currently in scope.  We return the first term with highest degree and the guessed degree.
+This happens in `extract_top_degree_terms_and_deg`.
+
+Now, `compute_degree_le` chains together a few lemmas to conclude.  It guesses that the degree of a
+sum of terms is at most the degree of each individual term.
+We start with a goal of the form `f.nat_degree ≤ d`.  Recurse into `f` breaking apart sums and
+products.  Take care of numerals, `C a, X (^ n), monomial a n` separately.
+
+_Heuristic:_ the terms of "apparent" highest degree do not cancel.
+
+Finally, `compute_degree` takes one extra step.  It isolates the term of highest guessed degree
+and assumes that all remaining terms have smaller degree.  It checks that the degree of the highest
+term is what it is claimed (and further assumes that the highest term is a pure `X`-power, `X ^ n`,
+a pure `X` term or a product of one of these by `C a` and checks that the assumption `a ≠ 0` is in
+context).
+`compute_degree` then outsources the rest of the computation to `compute_degree_le`, once the goal
+has been appropriately replaced.
+
+###  Error reporting
+The tactics report that
+* naturals involving variables are not allowed in exponents for `compute_deg`;
+* when a simple lemma application would have sufficed (via a `Try this: ...`);
+* when the guessed degree is incompatible with the goal, suggesting a sharper value.
+-/
+
+namespace polynomial
+variables {R : Type*} [semiring R] (a : polynomial R)
+
+/-- Useful to expose easy hypotheses:
+* `df` should be dealt with by `single_term_resolve`,
+* `dg` should be dealt with by `compute_degree_le`.
+-/
+lemma nat_degree_add_left_succ (n : ℕ) (f g : polynomial R)
+  (df : f.nat_degree = n.succ) (dg : g.nat_degree ≤ n) :
+  (f + g).nat_degree = n.succ :=
+by rwa nat_degree_add_eq_left_of_nat_degree_lt (dg.trans_lt (nat.lt_of_succ_le df.ge))
+
+lemma nat_degree_add_right_succ (n : ℕ) (f g : polynomial R)
+  (df : f.nat_degree ≤ n) (dg : g.nat_degree = n.succ) :
+  (f + g).nat_degree = n.succ :=
+by rwa nat_degree_add_eq_right_of_nat_degree_lt (df.trans_lt (nat.lt_of_succ_le dg.ge))
+
+lemma nat_degree_eq_of_le_of_coeff_ne_zero {n : ℕ} {f : polynomial R}
+  (fn : f.nat_degree ≤ n) (f0 : f.coeff n ≠ 0) :
+  f.nat_degree = n :=
+le_antisymm fn (le_nat_degree_of_ne_zero f0)
+
+lemma monic_of_le_of_coeff_eq_one [nontrivial R] {n : ℕ} {f : polynomial R}
+  (fn : f.nat_degree ≤ n) (f0 : f.coeff n = 1) :
+  f.monic :=
+begin
+  rw [monic, ← f0, leading_coeff],
+  congr,
+  refine nat_degree_eq_of_le_of_coeff_ne_zero fn (λ h, (one_ne_zero (f0.symm.trans h))),
+end
+
+lemma coeff_C_eq_zero_of_succ (n : ℕ) (a : R) :
+  (C a).coeff (n + 1) = 0 :=
+by simp [coeff_C]
+
+lemma nat_degree_eq_iff_le_and_coeff_ne_zero {n : ℕ} (n0 : n ≠ 0) (f : polynomial R) :
+  f.nat_degree = n ↔ f.nat_degree ≤ n ∧ f.coeff n ≠ 0 :=
+begin
+  refine ⟨_, λ ⟨fn, f0⟩, nat_degree_eq_of_le_of_coeff_ne_zero fn f0⟩,
+  rintro rfl,
+  exact ⟨rfl.le, leading_coeff_ne_zero.mpr (ne_zero_of_nat_degree_gt (nat.pos_of_ne_zero n0))⟩,
+end
+
+end polynomial
 
 namespace tactic
 namespace compute_degree
 open expr polynomial
+
+/--  If an expression `e` is an iterated suquence of `bit0` and `bit1` starting from `0` or `1`,
+then `num_to_nat e` returns `some n`, where `n` is the natural number obtained from the same
+sequence of `bit0` and `bit1` applied to `0` or `1`.  Otherwise, `num_to_nat e = none`. -/
+-- for the application, the line `| `(has_zero.zero) := some 0` step is unnecessary: the standard
+-- assumption is that the coefficient of the term of highest-looking term is non-zero.
+meta def num_to_nat : expr → option ℕ
+| `(has_zero.zero) := some 0
+| `(has_one.one)   := some 1
+| `(bit0 %%a)      := match num_to_nat a with
+  | some an        := some (bit0 an)
+  | none           := none
+  end
+| `(bit1 %%a)      := match num_to_nat a with
+  | some an        := some (bit1 an)
+  | none           := none
+  end
+| `(%%a + %%b)      := match num_to_nat a, num_to_nat b with
+  | (some an), (some bn) := some (an + bn)
+  | _, _ := none
+  end
+| `(%%a * %%b)      := match num_to_nat a, num_to_nat b with
+  | (some an), (some bn) := some (an * bn)
+  | _, _ := none
+  end
+| `(%%a ^ %%b)      := match num_to_nat a, num_to_nat b with
+  | (some an), (some bn) := some (an ^ bn)
+  | _, _ := none
+  end
+| _ := none
+
+/--  `convert_num_to_C_num a` takes an expression `a`, assuming that it is a term in a polynomial
+ring `R[X]`.  If `a` is an iterated application of `bit0` and `bit1` to `0` or `1`, then
+`convert_num_to_C_num` produces a proof of the equality
+`a = C (a : R)` and rewrites the goal with this identity.  Otherwise, the tactic does nothing. -/
+meta def convert_num_to_C_num (a : expr) : tactic unit :=
+match num_to_nat a with
+| (some an) := do
+  `(@polynomial %%R %%inst) ← infer_type a,
+  aexp ← to_expr ``(%%(reflect an)) tt ff,
+  n_eq_Cn ← to_expr ``(%%a = polynomial.C (%%aexp : %%R)),
+  (_, nproof) ← solve_aux n_eq_Cn
+    `[ simp only [nat.cast_bit1, nat.cast_bit0, nat.cast_one, C_bit1, C_bit0, map_one] ],
+  rewrite_target nproof
+| none := skip
+end
+
+/--  Let `e` be an expression.  Assume that `e` is
+* `C a * X (^ n)`,
+* `num * X (^ n)`, where `num` is a sequence of `bit0` and `bit1` applied to `1`,
+* `monomial n a`,
+* `X (^ n)`,
+in a polynomial ring over `R`.
+`single_term_resolve e` produces a proof of the goal `e.nat_degree = d`, where `d` is the
+exponent of `X`.
+
+Assumptions: the tactic tries to discharge the proof that constant in front of the power of `X` is
+non-zero using `assumption <|> ...`.
+When it is needed, `single_term_resolve` produces a `nontriviality` assumption using tactic
+`nontriviality R` or fails. -/
+meta def single_term_resolve : expr → tactic unit
+| `(has_mul.mul %%a %%X) := do
+  convert_num_to_C_num a,
+  refine ``(polynomial.nat_degree_C_mul_X _ _) <|>
+    refine ``(polynomial.nat_degree_C_mul_X_pow _ _ _) <|>
+    fail "The leading term is not of the form\n`C a * X (^ n)`\n\n",
+  assumption <|> interactive.exact ``(one_ne_zero) <|> skip
+| (app `(⇑(@polynomial.monomial %%R %%inst %%n)) x) := do
+  refine ``(polynomial.nat_degree_monomial_eq %%n _),
+  assumption <|> interactive.exact ``(one_ne_zero) <|> skip
+| (app `(⇑(@polynomial.C %%R %%inst)) x) :=
+  interactive.exact ``(polynomial.nat_degree_C _)
+| `(@has_pow.pow (@polynomial %%R %%nin) ℕ %%inst %%mX %%n) :=
+  (nontriviality_by_assumption R <|>
+    fail format!"could not produce a 'nontrivial {R}' assumption") >>
+  refine ``(polynomial.nat_degree_X_pow %%n)
+| `(@polynomial.X %%R %%inst) :=
+  (nontriviality_by_assumption R <|>
+    fail format!"could not produce a 'nontrivial {R}' assumption") >>
+  interactive.exact ``(polynomial.nat_degree_X)
+| e := do ppe ← pp e,
+  fail format!"'{ppe}' is not a supported term: can you change it to `C a * X (^ n)`?\n
+See the docstring of `tactic.compute_degree.single_term_resolve` for more shapes. "
+
 
 /--  `guess_degree e` assumes that `e` is an expression in a polynomial ring, and makes an attempt
 at guessing the `nat_degree` of `e`.  Heuristics for `guess_degree`:
@@ -64,6 +237,37 @@ meta def guess_degree : expr → tactic expr
 | e                          := do `(@polynomial %%R %%inst) ← infer_type e,
                                 pe ← to_expr ``(@nat_degree %%R %%inst) tt ff,
                                 pure $ expr.mk_app pe [e]
+
+/--  `eval_guessing n e` takes a natural number `n` and an expression `e` and gives an
+estimate for the evaluation of `eval_expr' ℕ e`.  It is tailor made for estimating degrees of
+polynomials.
+
+It decomposes `e` recursively as a sequence of additions, multiplications and `max`.
+On the atoms of the process, `eval_guessing` tries to use `eval_expr' ℕ`, resorting to using
+`n` if `eval_expr' ℕ` fails.
+
+For use with degree of polynomials, we mostly use `n = 0`. -/
+meta def eval_guessing (n : ℕ) : expr → tactic ℕ
+| `(%%a + %%b)   := (+) <$> eval_guessing a <*> eval_guessing b
+| `(%%a * %%b)   := (*) <$> eval_guessing a <*> eval_guessing b
+| `(max %%a %%b) := max <$> eval_guessing a <*> eval_guessing b
+| e              := eval_expr' ℕ e <|> pure n
+
+meta def guess_degree_to_nat : expr → ℕ
+| `(has_zero.zero)         := 0
+| `(has_one.one)           := 0
+| `(- %%f)                 := guess_degree_to_nat f
+| (app `(⇑polynomial.C) x) := 0
+| `(polynomial.X)          := 1
+| `(bit0 %%a)              := guess_degree_to_nat a
+| `(bit1 %%a)              := guess_degree_to_nat a
+| `(%%a + %%b)             := max (guess_degree_to_nat a) (guess_degree_to_nat b)
+| `(%%a - %%b)             := max (guess_degree_to_nat a) (guess_degree_to_nat b)
+| `(%%a * %%b)             := (guess_degree_to_nat a) + (guess_degree_to_nat b)
+| `(%%a ^ %%b)             := let bn := b.to_nat.get_or_else 0 in
+                              (guess_degree_to_nat a) * bn
+| (app `(⇑(polynomial.monomial %%n)) x) := n.to_nat.get_or_else 0
+| e                        := 0
 
 /-- `resolve_sum_step e` takes the type of the current goal `e` as input.
 It tries to make progress on the goal `e` by reducing it to subgoals.
@@ -115,20 +319,149 @@ with `c` a coefficient of the polynomial `f` in question. -/
 meta def norm_assum : tactic unit :=
 try `[ norm_num ] >> try assumption
 
-/--  `eval_guessing n e` takes a natural number `n` and an expression `e` and gives an
-estimate for the evaluation of `eval_expr' ℕ e`.  It is tailor made for estimating degrees of
-polynomials.
+meta def compute_step (deg : ℕ) : expr → tactic unit
+| `(%%l + %%r) := do [dle, dre] ← [l, r].mmap guess_degree,
+  [dl, dr] ← [dle, dre].mmap $ eval_guessing 0,
+  if dr < deg then do
+    --`[ rw polynomial.nat_degree_add_left_succ ]
+    refine ``(polynomial.nat_degree_add_left_succ _ %%l %%r _ _)
+  else
+  if dl < deg then do
+    --`[ rw polynomial.nat_degree_add_right_succ ]
+    refine ``(polynomial.nat_degree_add_right_succ _ %%l %%r _ _)
+  else
+    fail "sorry, there are two or more terms of highest expected degree"
+| _ := failed
 
-It decomposes `e` recursively as a sequence of additions, multiplications and `max`.
-On the atoms of the process, `eval_guessing` tries to use `eval_expr' ℕ`, resorting to using
-`n` if `eval_expr' ℕ` fails.
+/--  These are the cases in which an easy lemma computes the degree. -/
+meta def single_term_suggestions : tactic unit := do
+bo ← succeeds $ interactive.exact ``(polynomial.nat_degree_X_pow _),
+if bo then fail "Try this: exact polynomial.nat_degree_X_pow _"
+else do
+bo ← succeeds $ interactive.exact ``(polynomial.nat_degree_C _),
+if bo then fail "Try this: exact polynomial.nat_degree_C _"
+else do
+bo ← succeeds $ interactive.exact ``(polynomial.nat_degree_X),
+if bo then fail "Try this: exact polynomial.nat_degree_X"
+else do
+bo ← succeeds $ interactive.exact ``(polynomial.nat_degree_C_mul_X_pow _ _ ‹_›),
+if bo then fail "Try this: exact polynomial.nat_degree_C_mul_X_pow _ _ ‹_›"
+else do
+bo ← succeeds $ interactive.exact ``(polynomial.nat_degree_C_mul_X _ ‹_›),
+if bo then fail "Try this: exact polynomial.nat_degree_C_mul_X _ ‹_›"
+else
+  skip
+  --fail "'compute_degree' works better with polynomials involving more than one term\n"
 
-For use with degree of polynomials, we mostly use `n = 0`. -/
-meta def eval_guessing (n : ℕ) : expr → tactic ℕ
-| `(%%a + %%b)   := (+) <$> eval_guessing a <*> eval_guessing b
-| `(%%a * %%b)   := (*) <$> eval_guessing a <*> eval_guessing b
-| `(max %%a %%b) := max <$> eval_guessing a <*> eval_guessing b
-| e              := eval_expr' ℕ e <|> pure n
+/--  A simple check: `check_target_changes t` changes if `t` unifies with one of the current
+goals.  I use it to make sure that the tactics are actually making progress, by feeding the target
+`t`, stored before applying them. -/
+meta def check_target_changes (t : expr) : tactic unit :=
+do gs ← get_goals >>= list.mmap infer_type,
+  (success_if_fail $ gs.mfirst $ unify t) <|> fail "Goal did not change"
+
+/--  `compute_degree_le_core` differs from `compute_degree_le` simply since it takes a `bool`
+input, instead of parsing a `!` token. -/
+meta def compute_degree_le_core : tactic unit :=
+do t ← target,
+  try $ refine ``(polynomial.degree_le_nat_degree.trans (with_bot.coe_le_coe.mpr _)),
+  `(polynomial.nat_degree %%tl ≤ %%tr) ← target |
+    fail "Goal is not of the form\n`f.nat_degree ≤ d` or `f.degree ≤ d`",
+  expected_deg ← guess_degree tl >>= eval_guessing 0,
+  deg_bound ← eval_expr ℕ tr <|> pure expected_deg,
+  if deg_bound < expected_deg
+  then fail sformat!"the given polynomial has a term of expected degree\nat least '{expected_deg}'"
+  else
+    repeat $ target >>= resolve_sum_step,
+  check_target_changes t,
+  try $ any_goals' norm_assum
+
+meta def remove_one_coeff (fc : expr) : tactic unit :=
+do n ← get_unused_name "h",
+  R ← infer_type fc,
+  zer ← to_expr ``(0 : %%R) tt ff,
+  --az ← to_expr ``(add_zero (_ : %%R)) tt ff,
+  --za ← to_expr ``(zero_add (_ : %%R)) tt ff,
+  c0 ← mk_app `eq [fc, zer],
+  hc0 ← assert n c0,
+  refine ``(polynomial.coeff_eq_zero_of_nat_degree_lt (nat.lt_succ_of_le _)),
+  focus1 compute_degree_le_core,
+  interactive.rotate,
+  try $ rewrite_target hc0,
+  clear hc0
+  --,
+  --rewrite_target az <|> rewrite_target za
+
+meta def progressively_remove : tactic unit :=
+do `(%%a + %%b ≠ 0) ← target,
+  match b with
+  | `(polynomial.coeff %%pol %%n) := do de ← guess_degree pol, d ← eval_guessing 0 de,
+    nn ← eval_expr ℕ n,
+    if d < nn then
+      compute_degree.remove_one_coeff b
+    else skip
+  | _ := skip
+  end
+
+--  trace mapps,
+--  apps ← summ.mfilter (λ e : expr,
+--    do `(some %%arg) ← e.get_app_args.nth 3, darg ← guess_degree arg,
+--    narg ← eval_guessing 0 darg, return $ narg < 9 ),
+--  trace apps,
+--  trace "summ",summ.mmap (λ e : expr, e.get_app_fn) >>= trace,
+----  let small_deg := summ.mfilter
+----    (λ e : expr, let co:= e.get_fn_app in de ← guess_degree d, nd ← eval_guessing 0 de,
+----      return (nd < tar_deg : bool)),
+--    trace "*****************************",
+--    trace small_deg,
+--  (ne::rest) ← summ.mfilter
+--    (λ e, do de ← guess_degree e, nd ← eval_guessing 0 de, return (nd < tar_deg : bool)) |
+--       trace "nonono",
+--    trace ne,
+--  remove_one_coeff ne
+--  trace small_deg,
+--  gd ← summ.mmap guess_degree,
+--  nat_degs ← gd.mmap $ eval_guessing 0,trace nat_degs
+--  summands ← list_binary_operands
+--  lids ←
+
+
+meta def compute_degree_core (expos : bool) : tactic unit :=
+do t ← target,
+  try $ refine ``(polynomial.degree_le_nat_degree.trans (with_bot.coe_le_coe.mpr _)),
+  `(polynomial.nat_degree %%tl ≤ %%tr) ← target |
+    fail "Goal is not of the form\n`f.nat_degree ≤ d` or `f.degree ≤ d`",
+  exp_deg ← guess_degree tl >>= eval_guessing 0,
+  cond ← succeeds $ eval_expr ℕ tr,
+  deg_bou ← if cond then eval_expr ℕ tr else pure exp_deg,
+  if deg_bou < exp_deg
+  then fail sformat!"the given polynomial has a term of expected degree\nat least '{exp_deg}'"
+  else
+    repeat $ target >>= resolve_sum_step,
+  check_target_changes t
+    --,
+    --try $ any_goals' norm_assum
+
+/-- `extract_top_degree_terms_and_deg e` takes an expression `e` looks for summands in `e`
+(assuming the Type of `e` is `R[X]`), and produces the pairs `(e',deg)`, where `e'` is
+the list of summands of `e` of maximal guessed degree equal to `deg`.
+
+The tactic fails if `e` contains no summand (this probably means something else went wrong
+somewhere else). -/
+meta def extract_top_degree_terms_and_deg (e : expr) : tactic (list expr × ℕ) :=
+do te ← infer_type e,
+  ad ← to_expr ``((+) : %%te → %%te → %%te) tt ff,
+  summ ← list_binary_operands ad e,
+  gd ← summ.mmap guess_degree,
+  nat_degs ← gd.mmap $ eval_guessing 0,
+  let summ_and_degs := summ.zip nat_degs,
+  let max_deg := summ_and_degs.argmax (λ e : expr × ℕ, e.2),
+  match max_deg with
+  | none := fail
+      "'`compute_degree`' could not find summands: something has gone very wrong!\n\n"
+  | (some first) := return $
+    (prod.fst <$> summ_and_degs.filter (λ f : expr × ℕ, f.2 = first.2), first.2)
+  end
 
 end compute_degree
 
@@ -137,7 +470,6 @@ open compute_degree polynomial
 
 /--  `compute_degree_le` tries to solve a goal of the form `f.nat_degree ≤ d` or `f.degree ≤ d`,
 where `f : R[X]` and `d : ℕ` or `d : with_bot ℕ`.
-
 If the given degree `d` is smaller than the one that the tactic computes,
 then the tactic suggests the degree that it computed. -/
 meta def compute_degree_le : tactic unit :=
@@ -155,12 +487,276 @@ do t ← target,
       success_if_fail $ gs.mfirst $ unify t) <|> fail "Goal did not change",
     try $ any_goals' norm_assum
 
+meta def compute_degree_1 : tactic unit :=
+do try $ ( refine ``((polynomial.degree_eq_iff_nat_degree_eq_of_pos _).mpr _) >>
+    rotate ),
+   `(@polynomial.nat_degree %%R %%inst %%pol = %%deg) ← target,
+  refine ``(le_antisymm _ (polynomial.le_nat_degree_of_ne_zero _)),
+  focus1 ( compute_degree_le_core >> done ),
+  ad ← to_expr ``((+) : (%%R) → (%%R) → (%%R)) tt ff,
+--  trace deg, infer_type deg >>= trace,
+  tar_deg ← eval_expr ℕ deg,
+--trace tar_deg,
+--  summ ← list_binary_operands ad pol,trace summ,
+  `[ repeat { rw coeff_add } ],
+--  te ← infer_type pol,
+  --trace target,
+  --trace sum_coefs,
+  --trace "summ0",
+  --let napps := summ.map (λ e, (e.get_app_args.nth 2).get_or_else e),--trace napps,
+--  repeat (do
+--  target >>= trace,
+  `(%%sum_coefs ≠ %%z) ← target | fail "oyoyoy",
+  summ ← list_binary_operands ad sum_coefs,--trace summ,
+  trace "mapps",
+  mapps ← summ.mfilter (λ e, do
+    let f := (e.get_app_args.nth 2).get_or_else e,
+    gf ← (guess_degree f) ,
+    ef ← eval_guessing 0 gf,
+    return (ef < tar_deg : bool)),--trace mapps,
+  mapps.mmap' (λ x, try $ remove_one_coeff x),
+--  gs ← get_goals,
+--  gt ← gs.mmap infer_type,
+--  trace gt,
+--  target >>= trace,
+   --try $
+--    `[ simp [ polynomial.coeff_one ]],
+     try $ any_goals' `[ simp only [polynomial.coeff_C, polynomial.coeff_mul_X_pow',
+      polynomial.coeff_monomial, polynomial.coeff_bit0_mul, polynomial.coeff_bit1_mul,
+      polynomial.coeff_neg, zero_add, add_zero, polynomial.coeff_one, zero_eq_bit0, bit0_eq_zero,
+      if_false, neg_zero', add_zero, one_ne_zero, not_false_iff] ],
+  try $ any_goals' `[ norm_num ],
+--  gs ← get_goals,
+--  gt ← gs.mmap infer_type,
+--  trace gt,
+--  target >>= trace,trace gs.length,
+  --iterate_at_most 4 $ any_goals' norm_assum,
+    try $ any_goals' `[ simp only [polynomial.coeff_C, polynomial.coeff_one
+    , zero_eq_bit0, bit0_eq_zero, if_false, neg_zero', add_zero, one_ne_zero, not_false_iff
+    ]],
+    try $ any_goals' assumption
+
+/--  `compute_degree` tries to solve a goal of the form `f.nat_degree = d` or  `f.degree = d`,
+where `d : ℕ` and `f` satisfies:
+* `f` is a sum of expressions of the form
+  `C a * X ^ n, C a * X, C a, X ^ n, X, monomial n a, monomial n a * monomial m b`;
+* all exponents and the `n` in `monomial n a` are *closed* terms of type `ℕ`;
+* the term with largest exponent is `C a * X ^ n, X ^ n, C a * X, X, C a` and is the unique term of
+  its degree (repetitions are allowed in terms of smaller degree);
+* if the leading term involves a product with `C a`, there must be in context the assumption
+  `a ≠ 0`;
+* if the goal is computing `degree`, instead of `nat_degree`, then the expected degree `d` should
+  not be `⊥`.
+
+If the given degree does not match what the tactic computes,
+then the tactic suggests the degree that it computed.
+
+You can also pass an optional argument to `compute_degree`, letting the tactic know which term is
+the one of highest degree.  The syntax is `compute_degree [<expression for one term>]`.  The
+expression can involve underscore, and Lean will try to unify them with one of the summands in the
+goal.  This opens the possibility of working with polynomials whose exponents are not closed natural
+numbers, though this is mostly unimplemented still.
+
+The tactic also reports when it is used with non-closed natural numbers as exponents. -/
+meta def compute_degree : tactic unit :=
+do try $ ( refine ``((polynomial.degree_eq_iff_nat_degree_eq_of_pos _).mpr _) >>
+    rotate ),
+  single_term_suggestions,
+  t ← target,
+  `(@polynomial.nat_degree %%R %%inst %%pol = %%degv) ← target |
+  fail "Goal is not of the form\n`f.nat_degree = d` or `f.degree = d`",
+  gde ← guess_degree pol,
+  deg ← eval_guessing 0 gde,
+  degvn ← eval_expr ℕ degv,
+  guard (deg = degvn) <|>
+  ( do ppe ← pp deg, ppg ← pp degvn,
+    fail sformat!("'{ppe}' is the expected degree\n" ++ "'{ppg}' is the given degree\n") ),
+  ad ← to_expr ``(@has_add.add (@polynomial %%R %%inst)
+    (infer_instance : has_add (@polynomial %%R %%inst) )) tt ff,
+--  ad ← to_expr ``(has_add.add :
+--    (@polynomial %%R %%inst) → (@polynomial %%R %%inst) → (@polynomial %%R %%inst)) tt ff,
+  summ ← list_binary_operands ad pol,
+  --let top_degs := prod.mk tt <$> (summ.filter (λ t, guess_degree_to_nat t = deg)).map to_pexpr,
+  --let iters := summ.length - top_degs.length,
+  let low_degs := (prod.mk ff <$> (summ.filter (λ t, guess_degree_to_nat t < deg)).map to_pexpr),
+  let iters := low_degs.length,
+  trace iters,
+  move_op.with_errors (to_pexpr ad) low_degs none,target >>= trace,
+  iterate_at_most iters $
+  ( do `(polynomial.nat_degree %%po = _) ← target,
+    compute_step deg po ),
+  any_goals' $ try $
+    (do `(polynomial.nat_degree %%po = _) ← target, single_term_resolve po),
+  check_target_changes t,
+  any_goals' $ try $ compute_degree_le_core,
+--  `(polynomial.nat_degree %%pol = %%degv) ← target,
+  skip
+  --gs ← get_goals,
+  --gt ← gs.mmap infer_type,
+  --gt.mmap expr.instantiate_univ_params,
+--  try $ any_goals' norm_assum
+
+/--  `compute_degree.with_lead lead` assumes that `lead` is an expression for the highest degree
+term of a polynomial and proceeds to try to close a goal of the form
+`f.nat_degree = d` or `f.degree = d`. -/
+meta def _root_.tactic.compute_degree.with_lead_ (lead : expr) : tactic unit := do
+move_op.with_errors ``((+)) [(ff, pexpr.of_expr lead)] none,
+refine ``(polynomial.nat_degree_add_left_succ _ %%lead _ _ _) <|>
+  single_term_suggestions,
+single_term_resolve lead,
+gs ← get_goals,
+gts ← gs.mmap infer_type,
+-- `is_ineq` is a list of tactics, one for each goal:
+-- * if the goal has the form `f.nat_degree ≤ d`, the tactic is `compute_degree_le`
+-- * otherwise, it is the tactic that tries `norm_num` and `assumption`
+is_ineq ← gts.mmap (λ t : expr, do match t with
+  | `(polynomial.nat_degree %%_ ≤ %%_) := return $ compute_degree_le_core
+  | _                                  := return norm_assum end),
+focus' is_ineq
+
 add_tactic_doc
 { name := "compute_degree_le",
   category := doc_category.tactic,
   decl_names := [`tactic.interactive.compute_degree_le],
   tags := ["arithmetic, finishing"] }
 
+add_tactic_doc
+{ name := "compute_degree",
+  category := doc_category.tactic,
+  decl_names := [`tactic.interactive.compute_degree],
+  tags := ["arithmetic, finishing"] }
+
 end interactive
 
 end tactic
+
+/-
+#exit
+/--  `compute_degree.with_lead lead` assumes that `lead` is an expression for the highest degree
+term of a polynomial and proceeds to try to close a goal of the form
+`f.nat_degree = d` or `f.degree = d`. -/
+meta def _root_.tactic.compute_degree.with_lead (args : list expr) : tactic unit := do
+let larg := args.map (λ e, (ff, pexpr.of_expr e)),
+move_op.with_errors ``((+)) larg none,
+match args with
+| [] := fail "oops, no terms of top degree?"
+| (a::as) := do
+  `(@polynomial.nat_degree %%R %%inst %%pol = %%deg) ← target,
+  mad ← to_expr ``(has_add.add : polynomial %%R → polynomial %%R → polynomial %%R) tt ff,
+  meq ← to_expr ``((=) : ℕ → ℕ → Prop) tt ff,
+  mdeg ← to_expr ``(polynomial.nat_degree : polynomial %%R → ℕ) tt ff,
+  n ← get_unused_name "h",
+  --pR ← infer_type sum, --trace pR,
+  --pR ← instantiate_mvars pR, --trace pR,
+  summands ← pol.list_summands | skip,
+  (r::rs) ← summands.mfilter (λ e : expr, do farg ← args.mfilter (λ g : expr, succeeds $ unify e g),
+    return (farg.length = 0)) | skip,
+  (expr.const na ls) ← return pol.get_app_fn,
+  let sum := as.foldl (λ e, mad.mk_app [e]) a,
+  let sum := sum.instantiate_univ_params $ [na].zip ls,--trace "invs", trace sum,
+  trace "it sum",
+  its ← infer_type sum,
+  ppr ← to_expr ``(@polynomial %%R %%inst) tt ff,
+  trace $ succeeds $ unify its ppr,
+  let sum_rs := rs.foldl (λ e, mad.mk_app [e]) r,
+  let sum_rs := sum_rs.instantiate_univ_params $ [na].zip ls,--trace "invs", trace sum_rs,
+  let re_sum := mad.mk_app [sum_rs, sum],trace re_sum,
+  let re_sum := re_sum.instantiate_univ_params $ [na].zip ls,trace "re_sum", trace re_sum,
+  let top_deg := expr.mk_app mdeg [sum],
+--  unify pR `(@polynomial %%R %%inst),
+  top_eq ← mk_app `eq [top_deg, deg],
+  neq ← assert n top_eq,
+  rotate,
+  --(@expr.const tt na ls, es) ← return mdeg.get_app_fn_args,
+
+  --trace "ls mdeg", trace ls,trace mdeg,
+    --te ← infer_type e, instantiate_univ_params, unify te `(polynomial %%R),
+--  (@expr.const tt na ls, es) ← return sum.get_app_fn_args,trace "ls sum", trace ls,trace sum,
+  --ls.mmap infer_type >>= trace,
+
+  toph ← get_local n,
+  re_eq ← mk_app `eq [pol, re_sum],
+  --trace re_eq,
+  (_, prf) ← solve_aux re_eq (reflexivity <|> `[{ simp only [add_assoc], done }]), --trace prf,
+  --gs ← get_goals, gs.mmap infer_type >>= trace,
+  rewrite_target prf,
+  refine ``(polynomial.nat_degree_add_left_succ _ _ _ _ _) <|>
+    single_term_suggestions,
+  tactic.exact toph--,
+--  compute_degree_le_core ff
+--  `[ rw nat_degree_add_eq_left_of_nat_degree_lt ],
+--  rewrite_target toph
+--  rewrite_target neq
+  --trace prf
+--  let rest := summands.filter (λ e : expr, e ∈ args.mfilter (λ g : expr, succeeds $ unify e g)),
+--   trace rest
+
+--  rest ← summands.mfilter (λ f, succeeds $ unify f a), trace rest
+end
+--  let rest := summands.filter (λ e, e ∉ args), trace rest
+  --let sum_rest := (rest).foldl (λ e, mad.mk_app [e]) r, trace sum_rest,
+#check list.band
+--  repeat $ rewrite_target add_assoc (X + X + X)
+#eval [4,5].filter (∈ [4])
+#check list.remove_all
+/-
+refine ``(polynomial.nat_degree_add_left_succ _ %%lead _ _ _) <|>
+  single_term_suggestions,
+single_term_resolve lead,
+gs ← get_goals,
+gts ← gs.mmap infer_type,
+-- `is_ineq` is a list of tactics, one for each goal:
+-- * if the goal has the form `f.nat_degree ≤ d`, the tactic is `compute_degree_le`
+-- * otherwise, it is the tactic that tries `norm_num` and `assumption`
+is_ineq ← gts.mmap (λ t : expr, do match t with
+  | `(polynomial.nat_degree %%_ ≤ %%_) := return $ compute_degree_le_core ff
+  | _                                  := return norm_assum end),
+focus' is_ineq
+-/
+
+/--  `compute_degree` tries to solve a goal of the form `f.nat_degree = d` or  `f.degree = d`,
+where `d : ℕ` and `f` satisfies:
+* `f` is a sum of expressions of the form
+  `C a * X ^ n, C a * X, C a, X ^ n, X, monomial n a, monomial n a * monomial m b`;
+* all exponents and the `n` in `monomial n a` are *closed* terms of type `ℕ`;
+* the term with largest exponent is `C a * X ^ n, X ^ n, C a * X, X, C a` and is the unique term of
+  its degree (repetitions are allowed in terms of smaller degree);
+* if the leading term involves a product with `C a`, there must be in context the assumption
+  `a ≠ 0`;
+* if the goal is computing `degree`, instead of `nat_degree`, then the expected degree `d` should
+  not be `⊥`.
+
+If the given degree does not match what the tactic computes,
+then the tactic suggests the degree that it computed.
+
+You can also pass an optional argument to `compute_degree`, letting the tactic know which term is
+the one of highest degree.  The syntax is `compute_degree [<expression for one term>]`.  The
+expression can involve underscore, and Lean will try to unify them with one of the summands in the
+goal.  This opens the possibility of working with polynomials whose exponents are not closed natural
+numbers, though this is mostly unimplemented still.
+
+The tactic also reports when it is used with non-closed natural numbers as exponents. -/
+meta def compute_degree_old : parse opt_pexpr_list → tactic unit
+| [] := do is_deg ← succeeds $ refine ``((polynomial.degree_eq_iff_nat_degree_eq_of_pos _).mpr _) >>
+  interactive.rotate,
+  `(polynomial.nat_degree %%tl = %%tr) ← target |
+    fail "Goal is not of the form\n`f.nat_degree = d` or `f.degree = d`",
+  (lead, m') ← extract_top_degree_terms_and_deg tl,
+  td ← eval_expr ℕ tr,
+  if m' ≠ td then do
+    pptl ← pp tl, ppm' ← pp m',
+    if is_deg then
+      fail sformat!"should the degree be '{m'}'?"
+    else
+     fail sformat!"should the nat_degree be '{m'}'?"
+  else do
+    tactic.compute_degree.with_lead (lead)
+| [lead] := do `(polynomial.nat_degree %%tl = %%tr) ← target |
+    fail "Goal is not of the form\n`f.nat_degree = d` or `f.degree = d`",
+  tls ← tl.list_summands,
+  lead ← to_expr lead,
+  (lead :: hs) ← tls.mfilter $ λ e', succeeds $ unify lead e',
+  tactic.compute_degree.with_lead [lead]
+| _  := fail "'compute_degree' only accepts one leading term"
+
+-/
