test/compute_degree.lean
@@ -2,7 +2,180 @@ import tactic.compute_degree
 
 open polynomial
 open_locale polynomial
+universe u
+--set_option pp.all true
+--instance {F : Type*} [comm_semiring F] : has_add (polynomial F) := by refine polynomial.has_add
+example {F : Type*} [comm_semiring F] [nontrivial F] : nat_degree (1 + X : F[X]) = 1 :=
+by compute_degree
 
+/-
+example {F} [ring F] [nontrivial F] (a b c : F[X]) :
+  nat_degree (a + a : F[X]) = 0 :=
+begin
+  compute_degree,
+end
+-/
+example {F : Type*} [semiring F] (h2 : (2 : F) ≠ 0) : nat_degree (X + 1 + X + 1 : F[X]) = 0 + 1 :=
+begin
+  compute_degree,
+  rw ← two_mul,
+  compute_degree,
+  norm_num,
+  assumption,
+end
+
+example {F : Type*} [ring F] (h2 : (2 : F) ≠ 0) : degree (X ^ 4 + (- 3) + X ^ 4 : F[X]) = 4 :=
+begin
+  compute_degree,
+--  norm_num, --times out, but does not using `{F : Type u}` or `[semiring F]`.
+  rw ← two_mul,
+  compute_degree,
+  norm_num,
+  assumption,
+  norm_num,
+end
+open tactic
+#eval compute_degree.num_to_nat `((2 * 2 + 2) ^ 2)
+
+
+example {F : Type*} [ring F] (h37 : ((37 : ℕ) : F) ≠ 0) : nat_degree (((2 * 2 + 2) ^ 2 + 1) * X + 1 : F[X]) = 1 :=
+begin
+  compute_degree,
+  recover,
+  norm_num,
+end
+
+#exit
+example : (X ^ 4 + 1 + X ^ 4 : polynomial ℕ).nat_degree = 1 + 1 + 1 + 1 :=
+by {
+  compute_degree,
+  norm_num,  -- no timeout using `ℕ[X]`
+  move_add (1 : ℕ[X]),
+  }
+--#exit
+
+--set_option pp.all true
+/-
+--  with Type*
+F: Type ?l_1
+_inst_1: ring.{?l_1} F
+_inst_2: nontrivial.{?l_1} F
+⊢ @eq.{1} nat (@polynomial.nat_degree.{?l_1} F (@ring.to_semiring.{?l_1} F _inst_1) (@has_add.add.{?l_1} (@polynomial.{?l_1} F (@ring.to_semiring.{?l_1} F _inst_1)) (@infer_instance.{?l_1+1} (has_add.{?l_1} (@polynomial.{?l_1} F (@ring.to_semiring.{?l_1} F _inst_1))) (@polynomial.has_add.{?l_1} F (@ring.to_semiring.{?l_1} F _inst_1))) (@polynomial.X.{?l_1} F (@ring.to_semiring.{?l_1} F _inst_1)) (@polynomial.X.{?l_1} F (@ring.to_semiring.{?l_1} F _inst_1)))) (nat.succ (@has_zero.zero.{0} nat nat.has_zero))
+
+--  with Type u, before norm_num
+F: Type u
+_inst_1: ring.{u} F
+_inst_2: nontrivial.{u} F
+--  same
+⊢ @eq.{1} nat (@polynomial.nat_degree.{u} F (@ring.to_semiring.{u} F _inst_1) (@has_add.add.{u} (@polynomial.{u} F (@ring.to_semiring.{u} F _inst_1))
+
+-- differs 1
+(@infer_instance.{u+1} (has_add.{u} (@polynomial.{u} F (@ring.to_semiring.{u} F _inst_1))) (@polynomial.has_add.{u} F (@ring.to_semiring.{u} F _inst_1)))
+
+-- same
+(@polynomial.X.{u} F (@ring.to_semiring.{u} F _inst_1)) (@polynomial.X.{u} F (@ring.to_semiring.{u} F _inst_1))))
+
+-- differs 2
+(nat.succ (@has_zero.zero.{0} nat nat.has_zero))
+
+--  with Type u, after norm_num
+F: Type u
+_inst_1: ring.{u} F
+_inst_2: nontrivial.{u} F
+-- same
+⊢ @eq.{1} nat (@polynomial.nat_degree.{u} F (@ring.to_semiring.{u} F _inst_1) (@has_add.add.{u} (@polynomial.{u} F (@ring.to_semiring.{u} F _inst_1))
+
+-- differs 1
+(@polynomial.has_add.{u} F (@ring.to_semiring.{u} F _inst_1))
+
+-- same
+(@polynomial.X.{u} F (@ring.to_semiring.{u} F _inst_1)) (@polynomial.X.{u} F (@ring.to_semiring.{u} F _inst_1))))
+
+-- differs 2
+(@has_one.one.{0} nat nat.has_one)
+-/
+example {F : Type*} [ring F] [nontrivial F] : degree (X + 0 + X : F[X]) = 1 :=
+by {
+
+  compute_degree,
+  work_on_goal 2 { norm_num },
+  norm_num,
+--  work_on_goal 2 { exact zero_lt_one },
+--  norm_num,
+/-
+  norm_num,
+  simp only [polynomial.coeff_mul_X_pow', polynomial.coeff_monomial, polynomial.coeff_bit0_mul, polynomial.coeff_bit1_mul, polynomial.coeff_neg,
+    zero_add, add_zero, polynomial.coeff_one, zero_eq_bit0, bit0_eq_zero, if_false, neg_zero', add_zero, one_ne_zero, not_false_iff],
+  rw polynomial.coeff_one,
+  norm_num,
+  norm_num,
+  --norm_num,
+  squeeze_simp [coeff_one],
+  simp only [coeff_one, zero_eq_bit0, bit0_eq_zero, if_false, neg_zero', add_zero, one_ne_zero, not_false_iff],
+  {compute_degree.compute_degree_le_core ff},
+  refine (polynomial.nat_degree_one.le.trans (nat.zero_le _)),
+-/
+  }
+#exit
+example {F : Type*} [ring F] [nontrivial F] : degree (X ^ 4 + 4 + X ^ 4 + C (- 1) : F[X]) = 4 :=
+by {
+
+  compute_degree;
+  norm_num,
+/-
+  norm_num,
+  simp only [polynomial.coeff_mul_X_pow', polynomial.coeff_monomial, polynomial.coeff_bit0_mul, polynomial.coeff_bit1_mul, polynomial.coeff_neg,
+    zero_add, add_zero, polynomial.coeff_one, zero_eq_bit0, bit0_eq_zero, if_false, neg_zero', add_zero, one_ne_zero, not_false_iff],
+  rw polynomial.coeff_one,
+  norm_num,
+  norm_num,
+  --norm_num,
+  squeeze_simp [coeff_one],
+  simp only [coeff_one, zero_eq_bit0, bit0_eq_zero, if_false, neg_zero', add_zero, one_ne_zero, not_false_iff],
+  {compute_degree.compute_degree_le_core ff},
+  refine (polynomial.nat_degree_one.le.trans (nat.zero_le _)),
+-/
+  }
+#exit
+example {R} [semiring R] [nontrivial R] {a b c d e : R} :
+  nat_degree (monomial 5 c * monomial 1 c + monomial 7 d +
+  (C a * X ^ 0 + (C b * X ^ 5 + X ^ 10 + C c * X ^ 2) + --0 * X ^ 10 +
+  X ^ 4 * X ^ 5) + C e * X ^ 9 + monomial 9 10) = 10 :=
+begin
+  compute_degree,
+/-
+  simp only [coeff_mul_X_pow', coeff_monomial],
+  norm_num,
+
+  simp only [coeff_C_mul, coeff_X_pow_self, mul_one, map_bit0, ne.def,
+  coeff_mul_X_pow', bit1_le_bit1, bit0_le_bit0, nat.one_le_bit0_iff, nat.lt_one_iff, eq_self_iff_true,   if_true],
+-/
+end
+example {R} [semiring R] (a b c : R) (h3 : (3 : R) ≠ 0) (f g h : R[X]) :
+  (C a + X + monomial 3 3 : R[X]).nat_degree = 3 :=
+begin
+  compute_degree,
+end
+
+--#exit
+
+example {R} [semiring R] (a b c : R) (h3 : (3 : R) ≠ 0) (f g h : R[X]) :
+  (C a + X + 1 + C (c * 4 * a) * X ^ 2 + X + X + C 6 + monomial 3 3 + 1: R[X]).nat_degree = 3 :=
+begin
+  compute_degree,
+end
+
+/-- goal did not change
+set_option pp.all true
+example {F : Type*} [ring F] [nontrivial F] (a b c : F[X]) :
+  nat_degree (X + a + X : F[X]) = 1 :=
+begin
+  compute_degree,
+end
+--/
+
+/- From here
+This part should be better and about `compute_degree_le`. -/
 variables {R : Type*} [semiring R] {a b c d e : R}
 
 example {p : R[X]} {n : ℕ} {p0 : p.nat_degree = 0} :
@@ -36,10 +209,150 @@ example {F} [ring F] {a : F} {n : ℕ} (h : n ≤ 10) :
   nat_degree (X ^ n - C a * X ^ 10 : F[X]) ≤ 10 :=
 by compute_degree_le
 
-example {F} [ring F] {a : F} {n : ℕ} (h : n ≤ 10) :
-  nat_degree (X ^ n + C a * X ^ 10 : F[X]) ≤ 10 :=
-by compute_degree_le
+/-  To here. -/
+example {F} [ring F] [nontrivial F] : degree (X ^ 4 + C (- 1) : F[X]) = 4 :=
+by {
+  compute_degree,
+  }
+--#exit
+variables {R : Type*} [semiring R] {f g h : R[X]} {a b c d e : R}
 
+section tests_for_compute_degree
+
+example {n : ℕ} (h : 1 + n < 11) :
+  degree (X ^ 5 + (X * monomial n 1 + X * X) + C a + C a * X ^ 10) ≤ 10 :=
+begin
+  compute_degree_le,
+  exact nat.lt_succ_iff.mp h,
+end
+
+example (a0 : a ≠ 0) : nat_degree (C a * X ^ 2) = 2 :=
+begin
+--  success_if_fail_with_msg {compute_degree}
+--    "Try this: exact polynomial.nat_degree_C_mul_X_pow _ _ ‹_›",
+  exact polynomial.nat_degree_C_mul_X_pow _ _ ‹_›
+end
+
+example (a0 : a ≠ 0) : nat_degree (C a * X) = 1 :=
+begin
+--  success_if_fail_with_msg {compute_degree}
+--    "Try this: exact polynomial.nat_degree_C_mul_X _ ‹_›",
+  exact polynomial.nat_degree_C_mul_X _ ‹_›
+end
+
+example : nat_degree (C a) = 0 :=
+begin
+--  success_if_fail_with_msg {compute_degree}
+--    "Try this: exact polynomial.nat_degree_C _",
+  exact polynomial.nat_degree_C _
+end
+
+example {R : Type*} [ring R] (a : R) (h : -a ≠ 0) :
+  nat_degree (C a * X ^ 2 + 1 : polynomial R) = 2 :=
+by { compute_degree, exact neg_ne_zero.mp h }
+
+example {R : Type*} [ring R] (h : ¬ (2 : R) = 0) :
+  nat_degree (2 * X ^ 2 + 1 : polynomial R) = 2 :=
+by compute_degree
+
+/--  Alex's example. -/
+example [char_zero R] :
+  nat_degree (2 * X ^ 2 + 1 : polynomial R) = 2 :=
+by compute_degree
+
+example {R : Type*} [ring R] (h : ¬ (21 : R) = 0) :
+  nat_degree (21 * X ^ 2 + 1 : polynomial R) = 2 :=
+by compute_degree
+
+example {R : Type*} [ring R] (a : R) (h : -a ≠ 0) : nat_degree (C a * X + 1 : polynomial R) = 1 :=
+by { compute_degree, exact neg_ne_zero.mp h }
+
+/--  Michael's example. -/
+example {F} [field F] : nat_degree (X ^ 4 + C 1 : F[X]) = 4 :=
+by compute_degree
+
+example {F} [ring F] [nontrivial F] : degree (X ^ 4 + C (- 1) : F[X]) = 4 :=
+by {compute_degree,
+  }
+
+example {F} [field F] : nat_degree (C 1 * X ^ 4 + X + C 1 : F[X]) = 4 :=
+by compute_degree
+
+example {F} [field F] {a : F} (a0 : a ≠ 0) : nat_degree (C a * X + C 1 : F[X]) = 1 :=
+by compute_degree
+
+example {F} [field F] {a : F} (a0 : a ≠ 0) : nat_degree (C a * X ^ 2 + C 1 : F[X]) = 2 :=
+by compute_degree
+
+example (ha : a ≠ 0) : nat_degree (C a * X ^ 3 + C b * X ^ 2 + C c * X + C d) = 3 :=
+by compute_degree
+
+example (ha : a ≠ 0) : degree (C a * X ^ 3 + C b * X ^ 2 + C c * X + C d) = 3 :=
+begin
+  success_if_fail_with_msg {compute_degree_le}
+    "Goal is not of the form\n`f.nat_degree ≤ d` or `f.degree ≤ d`",
+  compute_degree,
+end
+
+section non_trivial_assumption
+variable [nontrivial R]
+
+example : nat_degree (monomial 5 c * monomial 1 c + monomial 7 d + monomial 9 1 +
+    C a * X ^ 0 + C b * X ^ 5 + C c * X ^ 2 + X ^ 10 + C e * X) = 10 :=
+by compute_degree
+
+example : nat_degree (X : R[X]) = 1 :=
+begin
+--  success_if_fail_with_msg {compute_degree}
+--    "Try this: exact polynomial.nat_degree_X",
+  exact polynomial.nat_degree_X
+end
+
+example : nat_degree (X ^ 4 : R[X]) = 4 :=
+begin
+--  success_if_fail_with_msg {compute_degree}
+--    "Try this: exact polynomial.nat_degree_X_pow _",
+  exact polynomial.nat_degree_X_pow _
+end
+
+example : nat_degree (X + 1 : polynomial R) = 1 :=
+by compute_degree
+
+example : nat_degree (C 1 * X + 1 : polynomial R) = 1 :=
+by compute_degree
+
+example : nat_degree (monomial 5 c * monomial 1 c + monomial 7 d + monomial 9 1 +
+    C a * X ^ 0 + C b * X ^ 5 + C c * X ^ 2 + X ^ 10 + C e * X) = 10 :=
+by compute_degree
+
+example : nat_degree (monomial 1 c + monomial 5 c * monomial 1 c + monomial 7 d + monomial 9 1 +
+    C a * X ^ 0 + C b * X ^ 5 + C c * X ^ 2 + X ^ 10 + C e * X) = 10 :=
+by compute_degree
+
+example : nat_degree (monomial 5 c * monomial 1 c + monomial 7 d +
+  C a * X ^ 0 + C b * X ^ 5 + C c * X ^ 2 + 0 * X ^ 10 + monomial 9 1 + C e * X) = 9 :=
+begin
+--  success_if_fail_with_msg {compute_degree}
+--    "'10' is the expected degree
+--'9' is the given degree
+--",
+  rw zero_mul,
+  compute_degree,
+end
+
+example [nontrivial R] : (monomial 5 c * monomial 1 c + monomial 7 d + monomial 9 1 +
+    C a * X ^ 0 + C b * X ^ 5 + C c * X ^ 2 + X ^ 10 + C e * X).nat_degree = 10 :=
+by compute_degree
+
+example : nat_degree (monomial 5 c * monomial 1 c + monomial 7 d +
+  C a * X ^ 0 + C b * X ^ 5 + C c * X ^ 2 + X ^ 10 + C e * X + bit0 0 : R[X]) = 10 :=
+begin
+  compute_degree,
+end
+
+end non_trivial_assumption
+example (n : ℕ) (h : 1 + n < 11) :
+  degree (X ^ n + (X * monomial n 1 + X * X) + C a + C a * X ^ 10) ≤ 10 :=
 example (n : ℕ) (h : 1 + n < 11) :
   degree (5 * X ^ n + (X * monomial n 1 + X * X) + C a + C a * X ^ 10) ≤ 10 :=
 begin
@@ -59,6 +372,17 @@ example : nat_degree (7 * X : R[X]) ≤ 1 :=
 by compute_degree_le
 
 example : (1 : polynomial R).nat_degree ≤ 0 :=
+begin
+--  success_if_fail_with_msg {compute_degree}
+--    "Goal is not of the form
+--`f.nat_degree = d` or `f.degree = d`",
+  compute_degree_le
+end
+
+example : (1 : polynomial R).nat_degree ≤ 0 :=
+by compute_degree_le
+
+example : nat_degree (C a * X ^ 3 + C b * X ^ 2 + C c * X + C d) ≤ 3 :=
 by compute_degree_le
 
 example : nat_degree (monomial 5 c * monomial 1 c + monomial 7 d +
@@ -76,6 +400,10 @@ end
 
 example : nat_degree (monomial 0 c * (monomial 0 c * C 1) + monomial 0 d + C 1 + C a * X ^ 0) ≤ 0 :=
 by compute_degree_le
+
+example {F} [ring F] {n m : ℕ} (n4 : n ≤ 4) (m4 : m ≤ 4) {a : F} :
+  nat_degree (C a * X ^ n + X ^ m + bit1 1 : F[X]) ≤ 4 :=
+by compute_degree_le; assumption
 
 example {F} [ring F] {n m : ℕ} (n4 : n ≤ 4) (m4 : m ≤ 4) {a : F} :
   nat_degree (C a * X ^ n + X ^ m + bit1 1 : F[X]) ≤ 4 :=
